src/tls/IK.fst
@@ -1,33 +1,33 @@
-module IK 
+module IK
 
 /// Standalone experiment modelling key extraction and key derivation
 /// parametrized by a usage function from labels to derived keyed
 /// functionalities.
 ///
 /// * captures resumption derivations via bounded-recursive instantiation.
-/// * captures PRF-ODH double game 
+/// * captures PRF-ODH double game
 /// * applied to the full extract/expand key schedule of TLS 1.3
 /// * models partial key compromise, controlled by the adversary for each new key
 /// * features agility on hash algorithms and DH groups, and ideal-only indexes.
 ///
 /// We plan to split this file into many modules, as planned on slack.
-/// 
+///
 /// Not done yet:
 ///
 /// * mysterious typing errors (see comments)
 ///
-/// * define/review all idealization flags. How are they accessed? 
-/// 
+/// * define/review all idealization flags. How are they accessed?
+///
 /// * reliance on u_of_i in DH extraction (intuitive but hard to code)
-/// 
-/// * key registration and discretionary compromise 
+///
+/// * key registration and discretionary compromise
 ///
 /// * extraction: ensure all strongly-dependent types disappear and
 ///   (concretely) the key schedule directly allocates all key
 ///   instances.
-/// 
+///
 /// * deal with create/coerce stateful pre- and post-condition.
-/// 
+///
 /// * usage restriction for KDFs, based on a generalization of wellformed_id
 ///   (starting with an example of hashed-log derivation)
 ///
@@ -38,12 +38,18 @@ module IK
 open FStar.HyperStack
 open FStar.HyperStack.ST
 
+module MM = MonotoneMap
+module MR = FStar.Monotonic.RRef
+module HH = FStar.HyperHeap
+
+let model = Flags.model
+
 // temporary imports
 
 type bytes = Platform.Bytes.bytes
 let lbytes (len:UInt32.t) = Platform.Bytes.lbytes (UInt32.v len)
 
-let sample (len:UInt32.t): ST (lbytes len) 
+let sample (len:UInt32.t): ST (lbytes len)
     (requires fun h0 -> True)
     (ensures fun h0 r h1 -> True)
   = CoreCrypto.random (UInt32.v len)
@@ -55,12 +61,18 @@ let sample (len:UInt32.t): ST (lbytes len)
 /// Index packages provide a "safe" predicate to control conditional idealization.
 /// We use "honest" to refer to the adversarie's intent, and "safe" for fine-grained idealization,
 /// with "safe ==> honest" as a pointwise lemma.
-/// When do we need to access one vs the other? Each instance can cache "safe". 
+/// When do we need to access one vs the other? Each instance can cache "safe".
 
-noeq type ipkg (info: Type0)  = | Idx: 
-  t: Type0 -> 
+noeq type ipkg (info: Type0)  = | Idx:
+  t: Type0 ->
+  r: MR.rid ->
   get_info: (t -> info) ->
-  honest: (t -> bool) ->  
+  honest: (i:t -> GTot Type0) ->
+  corrupt: (i:t -> GTot Type0) ->
+  get_honest: (i:t -> ST bool
+    (requires (fun _ -> True))
+    (ensures (fun h0 b h1 -> h0 == h1
+      /\ (b ==> honest i) /\ (not b ==> corrupt i)))) ->
   ipkg info
 
 /// Keyed functionality define Key packages, parametric in their
@@ -68,22 +80,23 @@ noeq type ipkg (info: Type0)  = | Idx:
 /// any number of other functions (such a leak, for instance).
 
 /// Derived key length restriction when using HKDF
-type keylen = l:UInt32.t {UInt32.v l <= 256} 
+type keylen = l:UInt32.t {UInt32.v l <= 256}
 
 // got into trouble using a type abbreviation [a:info{a == ip.get_info i}]; retry later; NS-11/03: Didn't understand this remark
 
 noeq type pkg (info: Type0) (ip: ipkg info) = | Pkg:
-  key: (ip.t -> Type0) -> 
+  key: (ip.t -> Type0) ->
   len: (info -> keylen) ->
+  ideal: Type0 -> // Type-level access to the ideal flag of the package
   create: (
     i:ip.t -> a:info{a == ip.get_info i} -> ST (key i)
-    (requires fun h0 -> True)
-    (ensures fun h0 p h1 -> True)) -> 
+    (requires fun h0 -> model)
+    (ensures fun h0 p h1 -> True)) ->
   coerce: (
     i:ip.t -> a:info{a == ip.get_info i} -> lbytes (len a) -> ST (key i)
-    (requires fun h0 -> ~(ip.honest i))
+    (requires fun h0 -> ideal ==> ip.corrupt i)
     (ensures fun h0 p h1 -> True)) ->
-  pkg info ip 
+  pkg info ip
 
 /// The "get_info" function ensure that all instances share the same
 /// runtime information; we still pass info inasmuch as the index will
@@ -92,10 +105,10 @@ noeq type pkg (info: Type0) (ip: ipkg info) = | Pkg:
 
 /// NEXT, WE DEFINE A FEW SAMPLE FUNCTIONALITIES,
 /// parameterized on their abstract index package.
-/// 
-/// can we factor out pre/post and boilerplate spec? 
 ///
-/// When ~(honest i), we must have  
+/// can we factor out pre/post and boilerplate spec?
+///
+/// When ~(honest i), we must have
 ///
 /// create i a == coerce i a (sample (len a))
 
@@ -113,28 +126,29 @@ let aeadLen: aeadAlg -> keylen = function
 // 17-10-31  this abbreviation breaks typechecking when used; why?
 // unfold type aeadAlgi (#ip:ipkg aeadAlg) (i:ip.t) = a:aeadAlg {a == ip.get_info i}
 
+assume val flag_Key: bool
+type idealKey = b2t flag_Key
+
 type keyrepr a = lbytes (aeadLen a)
 assume new type key (#ip: ipkg aeadAlg) (i: ip.t) // abstraction required for indexing
-assume val create_key: #ip: ipkg aeadAlg -> i: ip.t -> a:aeadAlg {a == ip.get_info i} -> 
+assume val create_key: #ip: ipkg aeadAlg -> i: ip.t -> a:aeadAlg {a == ip.get_info i} ->
   ST (key i)
-    (requires fun h0 -> True)
-    (ensures fun h0 p h1 -> True)  
+    (requires fun h0 -> model)
+    (ensures fun h0 p h1 -> True)
 
 assume val coerce_key: #ip: ipkg aeadAlg -> i: ip.t -> a:aeadAlg {a == ip.get_info i} -> keyrepr a ->
   ST (key i)
-    (requires fun h0 -> True)
+    (requires fun h0 -> idealKey ==> ip.corrupt i)
     (ensures fun h0 p h1 -> True)
 
-let mp (ip:ipkg aeadAlg): pkg aeadAlg ip = Pkg 
-  key 
-  aeadLen 
-  create_key 
+let mp (ip:ipkg aeadAlg): pkg aeadAlg ip = Pkg
+  key
+  aeadLen
+  idealKey
+  create_key
   coerce_key
 
-// NS:11/03: It's probably quite brittle for F* to infer ip
-//           It requires the type of the second argument to specifically be in
-//           the unreduced form Idx?.t ip
-val encrypt: #ip:ipkg aeadAlg -> #i:ip.t -> k: key i -> nat -> nat 
+val encrypt: #ip:ipkg aeadAlg -> #i:ip.t -> k: key i -> nat -> nat
 let encrypt #ip #i k v = v + 1
 
 /// --------------------------------------------------------------------------------------------------
@@ -142,80 +156,87 @@ let encrypt #ip #i k v = v + 1
 /// a default functionality (no idealization);
 /// for modelling, we could also provide a "leak" function
 
-type raw  (#ip: ipkg keylen) (i: Idx?.t ip) = lbytes (ip.get_info i)
-let create_raw (#ip: ipkg keylen) (i: ip.t) (len:keylen {len = ip.get_info i}): St (raw  i) = sample len
-let coerce_raw (#ip: ipkg keylen) (i: ip.t) (len:keylen {len = ip.get_info i}) (r:lbytes len): raw i = r
-let rp (ip:ipkg keylen): pkg keylen ip = Pkg 
-  raw 
-  (fun n -> n) 
-  create_raw 
-  coerce_raw
+assume val flag_Raw: bool
+type idealRaw = b2t flag_Raw
 
+type raw  (#ip: ipkg keylen) (i: Idx?.t ip) = lbytes (ip.get_info i)
+let create_raw (#ip: ipkg keylen) (i: ip.t) (len:keylen {len = ip.get_info i})
+  : ST (raw  i) (requires fun h0 -> model) (ensures fun h0 p h1 -> True) =
+  sample len
+let coerce_raw (#ip: ipkg keylen) (i: ip.t) (len:keylen {len = ip.get_info i}) (r:lbytes len)
+  : ST (raw i) (requires fun h0 -> idealRaw ==> ip.corrupt i)
+  (ensures fun h0 p h1 -> True) = r
+
+let rp (ip:ipkg keylen): pkg keylen ip = Pkg
+  raw
+  (fun n -> n)
+  idealRaw
+  create_raw
+  coerce_raw
 
 /// TLS-SPECIFIC KEY SCHEDULE
 /// --------------------------------------------------------------------------------------------------
 
 /// module Index
-/// 
+///
 /// We provide an instance of ipkg to track key derivation (here using constant labels)
 /// these labels are specific to HKDF, for now strings e.g. "e exp master".
 type label = string
 
 /// the middle extraction takes an optional DH secret, identified by this triple
 /// we use our own datatype to simplify typechecking
-type id_dhe = 
-  | NoIDH 
+type id_dhe =
+  | NoIDH
   | IDH:
-    #g: CommonDH.group -> 
-    gX: CommonDH.share g ->
-    gY: CommonDH.share g -> id_dhe
+    gX: CommonDH.dhi ->
+    gY: CommonDH.dhr gX -> id_dhe
 
-// The "ciphersuite hash algorithms"  eligible for TLS 1.3 key derivation. 
-// We will be more restrictive. 
+// The "ciphersuite hash algorithms"  eligible for TLS 1.3 key derivation.
+// We will be more restrictive.
 type kdfa = Hashing.Spec.alg
 
 /// Runtime key-derivation parameters, to be adjusted.
 ///
 /// HKDF defines an injective function from label * context to bytes, to be used as KDF indexes.
 ///
-type context = 
+type context =
   | Extract: context // TLS extractions have no label and no context; we may separate Extract0 and Extract2
-  | ExtractDH: id_dhe -> context // This is Extract1 (the middle extraction)
-  | Expand: context // TLS expansion with default hash value 
+  | ExtractDH: v:id_dhe -> context // This is Extract1 (the middle extraction)
+  | Expand: context // TLS expansion with default hash value
   | ExpandLog: // TLS expansion using hash of the handshake log
-    info: TLSInfo.logInfo (* ghost, abstract summary of the transcript *) -> 
+    info: TLSInfo.logInfo (* ghost, abstract summary of the transcript *) ->
     hv: Hashing.Spec.anyTag (* requires stratification *) -> context
 
 type id_psk = nat // external application PSKs only; we may also set the usage's maximal recursive depth here.
-type pre_id = 
-  | Preshared: 
-      a: kdfa (* fixing the hash algorithm *) -> 
-      id_psk  -> 
-      pre_id 
-  | Derive: 
-      i:pre_id (* parent index *) -> 
-      l:label (* static part of the derivation label *) -> 
-      context (* dynamic part of the derivation label *) -> 
+type pre_id =
+  | Preshared:
+      a: kdfa (* fixing the hash algorithm *) ->
+      id_psk  ->
+      pre_id
+  | Derive:
+      i:pre_id (* parent index *) ->
+      l:label (* static part of the derivation label *) ->
+      context (* dynamic part of the derivation label *) ->
       pre_id
 
 (* was:
   | Extract0: materials: pre_id -> pre_id
-  | Extract1: salt: pre_id -> materials: id_dhe -> pre_id 
+  | Extract1: salt: pre_id -> materials: id_dhe -> pre_id
   | Extract2: salt: pre_id -> pre_id
-  | Derived: 
-    secret:pre_id -> 
-    lbl: (* HKDF constant *) label -> 
-    info: TLSInfo.logInfo (* ghost, abstract summary of the transcript *) -> 
-    hv: Hashing.Spec.anyTag (* requires stratification *) -> pre_id 
+  | Derived:
+    secret:pre_id ->
+    lbl: (* HKDF constant *) label ->
+    info: TLSInfo.logInfo (* ghost, abstract summary of the transcript *) ->
+    hv: Hashing.Spec.anyTag (* requires stratification *) -> pre_id
 
-  | Derived: 
-    secret:pre_id -> 
-    lbl: (* HKDF constant *) label -> 
-    ctx: context -> 
-    pre_id 
-    
-    info: TLSInfo.logInfo (* ghost, abstract summary of the transcript *) -> 
-    hv: Hashing.Spec.anyTag (* requires stratification *) -> pre_id 
+  | Derived:
+    secret:pre_id ->
+    lbl: (* HKDF constant *) label ->
+    ctx: context ->
+    pre_id
+
+    info: TLSInfo.logInfo (* ghost, abstract summary of the transcript *) ->
+    hv: Hashing.Spec.anyTag (* requires stratification *) -> pre_id
 
 // We could have different constructors, depending on the presence of
 // a digest and length (in which case we should be careful of label
@@ -229,18 +250,15 @@ type pre_id =
 // prove that their encoding is injective.
 //
 // info is a function of hv, included for verification convenience.
-// (details to be adapted from the HS). 
+// (details to be adapted from the HS).
 // Hence same hashed digest ==> same logInfo, but not the converse.
 *)
 
-//17-10-30 painful
-// #set-options "--max_ifuel 3 --initial_ifuel 1"
-
 // always bound by the index (and also passed concretely at creation-time).
 val ha_of_id: i:pre_id -> kdfa
-let rec ha_of_id = function 
+let rec ha_of_id = function
   | Preshared a _ -> a
-  | Derive i lbl ctx -> ha_of_id i 
+  | Derive i lbl ctx -> ha_of_id i
 
 // placeholders
 assume val idh_of_log: TLSInfo.logInfo -> id_dhe
@@ -248,32 +266,150 @@ assume val summary: bytes -> TLSInfo.logInfo
 
 // concrete transcript digest
 let digest_info (a:kdfa) (info:TLSInfo.logInfo) (hv: Hashing.Spec.anyTag) =
-  exists (transcript: bytes). 
+  exists (transcript: bytes).
     // Bytes.length hv = tagLen a /\
-    hv = Hashing.Spec.hash a transcript /\ 
+    hv = Hashing.Spec.hash a transcript /\
     Hashing.CRF.hashed a transcript /\
-    info = summary transcript 
+    info = summary transcript
 
 /// stratified definition of id required.
 ///
 /// we will enforce
 /// * consistency on the hash algorithm
-/// * monotonicity of the log infos (recursively including earlier resumption logs). 
+/// * monotonicity of the log infos (recursively including earlier resumption logs).
 /// * usage restriction: the log after DH must include the DH identifier of the parent.
 ///   (Hence, we should either forbid successive DHs or authenticate them all.)
-/// 
-val wellformed_id: pre_id -> Type0 
+///
+val wellformed_id: pre_id -> Type0
 let rec wellformed_id = function
   | Preshared a _ -> True
-  | Derive i l (ExpandLog info hv) -> wellformed_id i /\ digest_info (ha_of_id i) info hv 
-  | Derive i lbl ctx -> 
-      //TODO "ctx either extends the parent's, or includes its idh" /\ 
-      wellformed_id i 
-           
+  | Derive i l (ExpandLog info hv) -> wellformed_id i /\ digest_info (ha_of_id i) info hv
+  | Derive i lbl ctx ->
+      //TODO "ctx either extends the parent's, or includes its idh" /\
+      wellformed_id i
+
 type id = i:pre_id {wellformed_id i}
 
+type honest_idh (c:context) =
+  ExtractDH? c /\ IDH? (ExtractDH?.v c) /\
+  (let ExtractDH (IDH gX gY) = c in CommonDH.honest_dhr gY)
 
-// 17-10-21 WIDE/NARROW INDEXES (old) 
+// ADL: we use a global honesty table for all indexes
+// Inside ipkg, we assume all index types are defined in the table below
+// We assume write access to this table is public, but the following global
+// invariant must be enforced: if i is corrupt then all indexes derived from i
+// are also corrupt - EXCEPT if ctx is ExtractDH g gx gy with CommonDH.honest_dhr gy
+let honest_region:MR.rid = new_region HH.root
+type honesty_invariant (m:MM.map' id (fun _ -> bool)) =
+  (forall (i:id) (l:label) (c:context{wellformed_id (Derive i l c)}).
+  {:pattern (m (Derive i l c))}
+  Some? (m (Derive i l c)) ==> Some? (m i) /\
+  (m i = Some false ==> (honest_idh c \/ m (Derive i l c) = Some false)))
+
+private type i_honesty_table =
+  MM.t honest_region id (fun (t:id) -> bool) honesty_invariant
+private let h_table = if model then i_honesty_table else unit
+
+let honesty_table: h_table =
+  if model then
+    MM.alloc #honest_region #id #(fun _ -> bool) #honesty_invariant
+  else ()
+
+// Registered is monotonic
+type registered (i:id) =
+  (if model then
+    let log : i_honesty_table = honesty_table in
+    MR.witnessed (MM.defined log i)
+  else True)
+
+type regid = i:id{registered i}
+
+type honest (i:regid) =
+  (if model then
+    let log : i_honesty_table = honesty_table in
+    MR.witnessed (MM.contains log i true)
+  else False)
+
+type corrupt (i:regid) =
+  (if model then
+    let log : i_honesty_table = honesty_table in
+    MR.witnessed (MM.contains log i false)
+  else True)
+
+// ADL: difficult to prove, see CommonDH for details
+let lemma_honest_corrupt (i:regid)
+  : Lemma (honest i <==> ~(corrupt i)) =
+  admit()
+
+let lemma_corrupt_invariant (i:regid) (lbl:label)
+  (ctx:context {wellformed_id (Derive i lbl ctx) /\ registered (Derive i lbl ctx)})
+  : ST unit
+  (requires fun h0 -> ~(honest_idh ctx))
+  (ensures fun h0 _ h1 ->
+    corrupt i ==> corrupt (Derive i lbl ctx) /\ h0 == h1)
+  =
+  lemma_honest_corrupt i;
+  lemma_honest_corrupt (Derive i lbl ctx);
+  if model then
+    let log : i_honesty_table = honesty_table in
+    MR.m_recall log;
+    MR.testify (MM.defined log i);
+    match MM.lookup log i with
+    | Some true -> ()
+    | Some false ->
+      let m = MR.m_read log in
+      // No annotation, but the proof relies on the global log invariant
+      MR.testify (MM.defined log (Derive i lbl ctx));
+      MM.contains_stable log (Derive i lbl ctx) false;
+      MR.witness log (MM.contains log (Derive i lbl ctx) false)
+  else ()
+
+let get_honest (i:regid) : ST bool
+  (requires fun h0 -> True)
+  (ensures fun h0 b h1 -> h0 == h1
+    /\ (b <==> honest i) /\ (not b <==> corrupt i))
+  =
+  lemma_honest_corrupt i;
+  if model then
+    let log : i_honesty_table = honesty_table in
+    MR.m_recall log;
+    MR.testify (MM.defined log i);
+    match MM.lookup log i with
+    | Some b -> b
+  else false
+
+// TODO(adl) preservation of the honesty table invariant
+let rec lemma_honesty_update (m:MM.map id (fun _ -> bool) honesty_invariant)
+  (i:regid) (l:label) (c:context{wellformed_id (Derive i l c)})
+  (b:bool{b <==> honest i /\ not b <==> corrupt i})
+  : Lemma (honesty_invariant (MM.upd m (Derive i l c) b))
+  = admit()
+
+let register_derive (i:regid) (l:label) (c:context{wellformed_id (Derive i l c)})
+  : ST (regid * bool)
+  (requires fun h0 -> True)
+  (ensures fun h0 (i', b) h1 ->
+    modifies_one honest_region h0 h1
+    /\ (i' == Derive i l c)
+    /\ (b2t b <==> honest i')
+    /\ (not b <==> corrupt i'))
+  =
+  let i':id = Derive i l c in
+  if model then
+    let log : i_honesty_table = honesty_table in
+    MR.m_recall log;
+    match MM.lookup log i' with
+    | Some b -> lemma_honest_corrupt i'; (i', b)
+    | None ->
+      let b = get_honest i in
+      let h = get () in
+      lemma_honesty_update (MR.m_sel h log) i l c b;
+      MM.extend log i' b;
+      lemma_honest_corrupt i';
+      (i', b)
+  else (i', false)
+
+// 17-10-21 WIDE/NARROW INDEXES (old)
 //
 // We'd rather keep wide indexes secret.  Internally, for each salt
 // index, we maintain a table from (g, gX, gY) to PRFs, with some
@@ -286,8 +422,9 @@ type id = i:pre_id {wellformed_id i}
 // this does not matter because security does not depend on their
 // sharing.
 
-assume val honest: i:id -> bool //17-10-31 FIXME
-let ii (#info:Type0) (get_info: id -> info) = Idx id get_info honest
+let ii (#info:Type0) (get_info: id -> info) =
+  Idx regid honest_region get_info honest corrupt get_honest
+
 /// Try out on examples: we may need a stateful invariant of the form
 /// "I have used this secret to create exactly these keys".
 
@@ -295,13 +432,32 @@ let ii (#info:Type0) (get_info: id -> info) = Idx id get_info honest
 /// We expect this function to be fully applied at compile time,
 /// returning a package and a algorithm-derivation function to its
 /// agility parameter (to be usually applied at run-time).
-/// 
+///
+
+/// ADL: PROPOSED CHANGE (09/11/17)
+/// ===================================================================================
+/// We propose to encode the idealization order of packages inside the usage function
+/// Namely, for all labels, the associated derived package can only be ideal if
+/// its parent is ideal. This condition will be checked when the packages are created
+/// (the packager must provide a flag that satisfies this condition), after the
+/// derivation tree is fixed.
+/// ===================================================================================
+/// noeq type range (info: Type0) (lbl:label) (ideal: Type0) = | Use:
+///     info': Type0 ->
+///     get_info': (id -> info') ->
+///     pkg': pkg info' (ii #info' get_info'){pkg'.ideal ==> ideal} ->
+///     derive: (i: id -> a: info -> ctx: context {wellformed_id (Derive i lbl ctx)} -> a': info' {a' == get_info' (Derive i lbl ctx)}) ->
+///     range info lbl
+///
+/// type usage (info: Type0) = (| ideal:Type0 & lbl: label -> (* compile-time *) range info lbl parent_ideal |)
+/// ===================================================================================
 
 noeq type range (info: Type0) (lbl:label) = | Use:
     info': Type0 ->
     get_info': (id -> info') ->
-    pkg': pkg info' (ii #info' get_info') -> 
-    derive: (i: id -> a: info -> ctx: context {wellformed_id (Derive i lbl ctx)} -> a': info' {a' == get_info' (Derive i lbl ctx)}) -> range info lbl
+    pkg': pkg info' (ii #info' get_info') ->
+    derive: (i: id -> a: info -> ctx: context {wellformed_id (Derive i lbl ctx)} -> a': info' {a' == get_info' (Derive i lbl ctx)}) ->
+    range info lbl
 
 type usage (info: Type0) = lbl: label -> (* compile-time *) range info lbl
 
@@ -309,29 +465,29 @@ type usage (info: Type0) = lbl: label -> (* compile-time *) range info lbl
 // invariant through extractions and derivations... until the first
 // hashed transcript, at which point the
 
-(* 
+(*
 /// parametricity? (Old/Later)
-/// we have [#id #pd #u #i #a] 
-/// u v returns [#ip #p (derive_alg: pd.info -> p.info) (derive_index: id.t -> i.t)] 
+/// we have [#id #pd #u #i #a]
+/// u v returns [#ip #p (derive_alg: pd.info -> p.info) (derive_index: id.t -> i.t)]
 ///
 /// We finally use a global, recursive instantiation of indexes to
 /// compose all our functionalities, with for instance
 /// (fun i -> Derived i v) to get the derived index.
 
-// (*UNUSED *) type usage' (#ii:ipkg) (a: ii.t -> Type0) = 
-//   label -> 
-//     ip:ipkg & 
-//     p: pkg ip & 
+// (*UNUSED *) type usage' (#ii:ipkg) (a: ii.t -> Type0) =
+//   label ->
+//     ip:ipkg &
+//     p: pkg ip &
 //     derive_index: (ii.t -> ip.t) &
 //     derive_info: (i: ii.t -> a i -> p.use (derive_index i))
 // note that [a] is [d.use]
 // should usage be part of info?
-// what about state state (safety etc)? 
+// what about state state (safety etc)?
 *)
 
 /// --------------------------------------------------------------------------------------------------
 /// module KDF
-/// 
+///
 /// we define a KDF parametric in both its usage and ipkg
 /// We rely on type abstraction to separate secrets with different indexes
 /// For soundness, we must also prevent external calls to create derived secrets.
@@ -339,100 +495,126 @@ type usage (info: Type0) = lbl: label -> (* compile-time *) range info lbl
 /// We idealize KDF as a random function, with lazy sampling.
 /// This holds syntactically only after inlining all calls to
 /// pkg.create/coerce.
-/// 
+///
 /// This requires memoizing calls, which is a bit tricky when calling
 /// stateful allocators.
 
-type details (ha:kdfa) = | Log: 
-  loginfo: TLSInfo.logInfo -> 
+assume val flag_KDF: b:bool{b ==> model}
+type idealKDF = b2t flag_KDF
+
+// Note that when model is off, safeKDF is False and corruptKDF is True
+type safeKDF (i:regid) = idealKDF /\ honest i
+type corruptKDF (i:regid) = idealKDF ==> corrupt i
+
+type details (ha:kdfa) = | Log:
+  loginfo: TLSInfo.logInfo ->
   hv: Hashing.Spec.anyTag {digest_info ha loginfo hv} -> details ha
 
 type info = | Info:
   ha:kdfa ->
-  option (details  ha) -> info 
+  option (details  ha) -> info
 
-val get_info: id -> info 
-#set-options "--initial_ifuel 2 --initial_fuel 2"
-let rec get_info (i0: id): info = 
-  match i0 with 
-  | Preshared a _ ->
-    Info a None 
-  
+// TODO find a nice way to express the idealization ordering
+assume val lemma_ideal_order: u:usage info -> lbl:label
+  -> Lemma (let use = u lbl in use.pkg'.ideal ==> idealKDF)
+
+val get_info: id -> info
+// 17-11-01 can't get it to verify; should follow from the definition of wellformed_id?
+let rec get_info (i0: id): info =
+  match i0 with
+  | Preshared a _ -> Info a None
   | Derive i l (ExpandLog log hv) ->
-    Info (ha_of_id i) (Some (Log log hv))
-
-  | Derive i _ _ -> 
-    get_info i 
-
-(* NS: USED TO BE WHAT FOLLOWS ...
-      
-   This indeed does not verify, 
-   since it seems to be off by a use of ha_of_id
-
-   Not sure what the intended semantics is 
-
-CF: still don't get it. second case was: 
-
-   | Derive i l (ExpandLog log hv) ->
+       assert(wellformed_id i0);
+       assume false;
+       // assert(wellformed_id i);
        let i:id = i in // sigh
        let Info a _ = get_info i in
        Info a (Some (Log log hv))
+  | Derive i _ _ ->
+       assert(wellformed_id i);
+       let i:id = i in // sigh
+       get_info i
 
-**)
-let derived_key 
-  (u: usage info) 
-  (i: id) 
+let derived_key
+  (u: usage info)
+  (i: regid)
   (lbl: label)
-  (c: context {wellformed_id (Derive i lbl c)})
-= 
-  let use = u lbl in 
-  let i': id = Derive i lbl c in 
+  (c: context {wellformed_id (Derive i lbl c) /\ registered (Derive i lbl c)})
+=
+  let use = u lbl in
+  let i' = Derive i lbl c in
   use.pkg'.key i'
 
-let there: FStar.Monotonic.RRef.rid = admit() 
+let there: MR.rid = admit()
 
 /// key-derivation table (memoizing create/coerce)
-type domain (i: id) = | Domain:
-  lbl: label -> 
-  ctx: context {wellformed_id (Derive i lbl ctx)} -> domain i 
+type domain (i:regid) = | Domain:
+  lbl: label ->
+  ctx: context {wellformed_id (Derive i lbl ctx) /\ registered (Derive i lbl ctx)} -> domain i
 
-private type table 
-  // (ip: ipkg) 
+type ideal_or_real (it:Type0) (rt:Type0) =
+  | Ideal: v:it -> ideal_or_real it rt
+  | Real: v:rt -> ideal_or_real it rt
+
+unfold type ir_key (safe: regid -> GTot Type0) (it:Type0) (rt:Type0) (i:regid) =
+  (if model then
+    s:ideal_or_real it rt{safe i <==> Ideal? s}
+  else rt)
+
+private type table
+  // (ip: ipkg)
   (u: usage info)
-  (i: id) 
+  (i: regid)
 = MonotoneMap.t there (domain i) (fun (Domain lbl ctx) -> derived_key u i lbl ctx) (fun _ -> True)
 
 let secret_len (a: info): keylen = UInt32.uint_to_t (Hashing.Spec.tagLen a.ha)
- 
-// when to be parametric on ip? not for the KDF itself: we use ip's constructors.
-let secret (u: usage info) (i: id) 
-=
-  if honest i 
-  then table u i 
-  else lbytes (secret_len (get_info i))
+type real_secret (i:regid) = lbytes (secret_len (get_info i))
 
-let secret_ideal (#u: usage info) (#i: id) (t: secret u i {honest i}): table u i = t 
-let ideal_secret (#u: usage info) (#i: id) (t: table u i {honest i}): secret u i = t 
-//let corrupt_secret (#u: usage info) (#i: id) (v: lbytes (secret_len (get_info i)) {~(honest i)}): secret u i = v
+type secret (u: usage info) (i:regid) =
+  ir_key safeKDF (table u i) (real_secret i) i
+
+// when to be parametric on ip? not for the KDF itself: we use ip's constructors.
+//type secret (u: usage info) (i:regid) =
+//  (if honest i then table u i
+//  else lbytes (secret_len (get_info i)))
+
+let secret_ideal (#u: usage info) (#i: regid) (t: secret u i {safeKDF i}): table u i =
+  let t : s:ideal_or_real (table u i) (real_secret i) {safeKDF i <==> Ideal? s} = t in
+  Ideal?.v t
+
+let ideal_secret (#u: usage info) (#i: regid) (t: table u i {safeKDF i}) : secret u i =
+  let t : s:ideal_or_real (table u i) (real_secret i) {safeKDF i <==> Ideal? s} = Ideal t in
+  assert(model); t
+
+let secret_corrupt (#u: usage info) (#i: regid) (t: secret u i {corruptKDF i}): real_secret i =
+  if model then
+   let t : s:ideal_or_real (table u i) (real_secret i) {safeKDF i <==> Ideal? s} = t in
+   (lemma_honest_corrupt i; Real?.v t)
+  else t
+
+let corrupt_secret (#u: usage info) (#i: regid) (t: real_secret i {corruptKDF i}) : secret u i =
+  if model then
+    (lemma_honest_corrupt i;
+    let s : s:ideal_or_real (table u i) (real_secret i) {safeKDF i <==> Ideal? s} = Real t in s)
+  else t
 
 /// Real KDF schemes, parameterized by an algorithm computed from the
 /// index (existing code).
- 
+
 /// maybe reverse-inline sampling from low-level KeyGen?
 /// otherwise we have to argue it is what Create does.
 ///
 /// MK: what does reverse-inline of low-level KeyGen mean?
 
-val coerce: 
-//ip: ipkg ->
+val coerce:
   u: usage info ->
-  i: id ->
-  a: info {a == get_info i} (* run-time *) -> 
-  repr: lbytes (secret_len a) -> 
+  i: regid ->
+  a: info {a == get_info i} (* run-time *) ->
+  repr: lbytes (secret_len a) ->
   ST (secret u i)
-  (requires fun h0 -> ~(honest i))
+  (requires fun h0 -> idealKDF ==> corrupt i)
   (ensures fun h0 p h1 -> True)
-let coerce u i a repr = repr
+let coerce u i a repr = corrupt_secret #u #i repr
 
 /// NS:
 /// MonotoneMap.alloc is a stateful function with all implicit arguments
@@ -451,74 +633,84 @@ let alloc (#r:FStar.Monotonic.RRef.rid) #a #b #inv (u:unit)
     inv (MonotoneMap.empty_map a b) /\
     ralloc_post r (MonotoneMap.empty_map a b) h0 (FStar.Monotonic.RRef.as_hsref x) h1))
   = MonotoneMap.alloc #r #a #b #inv
-  
-val create: 
+
+val create:
 //ip: ipkg ->
-  u: usage info -> 
-  i: id ->
+  u: usage info ->
+  i: regid ->
   a: info {a == get_info i}(* run-time *) ->
   ST (secret u i)
-  (requires fun h0 -> True)
+  (requires fun h0 -> model)
   (ensures fun h0 r h1 -> True)
-let create u i a = 
-  if honest i 
-  then 
-    ideal_secret (alloc ())
-  else 
-    coerce u i a (sample (secret_len a)) 
+let create u i a =
+  let honest = get_honest i in
+  if flag_KDF && honest then
+    let t : table u i = MonotoneMap.alloc #there #(domain i) #(fun (Domain lbl ctx) -> derived_key u i lbl ctx) #(fun _ -> True) in
+    ideal_secret t
+  else
+    corrupt_secret #u #i (sample (secret_len a))
 
 /// We are using many KDF packages (one for each usage),
 /// idealized one at a time.  (Having one proof step for each nested
 /// level of key derivation seems unavoidable: we need to idealize
 /// parents before childrens.)
 
-let pp (* ip:ipkg *) (u: usage info): pkg info (ii get_info) = Pkg 
-  (secret u) 
+let pp (* ip:ipkg *) (u: usage info): pkg info (ii get_info) = Pkg
+  (secret u)
   secret_len
-  (create u) 
+  idealKDF
+  (create u)
   (coerce u)
 
+let ukey (u:usage info) (lbl:label) (i':regid) =
+  let use = u lbl in
+  use.pkg'.key i'
+
 /// The well-formedness condition on the derived label (opaque from
-/// the viewpoint of the KDF) enforces 
-/// 
+/// the viewpoint of the KDF) enforces
+///
 inline_for_extraction
 val derive:
   #u: usage info ->
-  #i: id ->
-  a: info {a == get_info i} -> 
+  #i: regid ->
+  a: info {a == get_info i} ->
   k: secret u i ->
-  lbl: label -> 
-  ctx: context {wellformed_id (Derive i lbl ctx)} ->
-  ST (derived_key u i lbl ctx)
+  lbl: label ->
+  ctx: context {~(honest_idh ctx) /\ wellformed_id (Derive i lbl ctx)} ->
+  ST (i':regid{i' = Derive i lbl ctx} & ukey u lbl i')
   (requires fun h0 -> True)
   (ensures fun h0 r h1 -> True
     // modifies our own local state and whatever create/coerce modifies
     // no need to track the ideal state
   )
 
-let derive #u #i a k lbl ctx = 
-  let x = Domain lbl ctx in 
-  let use = u lbl in 
-  let a' = use.derive i a ctx in 
-  let i' = Derive i lbl ctx in 
-  if (* Flags.kdf n && *) honest i (*safe?*) 
+let derive #u #i a k lbl ctx =
+  // register (Derive i lbl ctx) and return its honesty (defaults to get_honest i)
+  let honest = get_honest i in
+  let i', honest' = register_derive i lbl ctx in
+  lemma_corrupt_invariant i lbl ctx;
+  let x = Domain lbl ctx in
+  let use = u lbl in
+  lemma_ideal_order u lbl; // TODO(adl) get the idealization order condition from (u lbl) above
+  let a' = use.derive i a ctx in
+  if flag_KDF && honest
   then
-    let v: option (derived_key u i lbl ctx) = MonotoneMap.lookup (secret_ideal k) x in 
-    match v with 
+    let v: option (derived_key u i lbl ctx) = MonotoneMap.lookup (secret_ideal k) x in
+    match v with
     //17-10-30 was failing with scrutiny error: match MonotoneMap.lookup (secret_ideal k) x
-    | Some dk -> dk
-    | None -> 
-      let dk = use.pkg'.create i' a' in 
+    | Some dk -> (| i', dk |)
+    | None ->
+      let dk = use.pkg'.create i' a' in
       //17-10-20 TODO framing across create
-      let h = HyperStack.ST.get() in 
-      assume(MonotoneMap.fresh (secret_ideal k) x h);
-      MonotoneMap.extend (secret_ideal k) x dk; 
-      dk
-  else 
+      let h = get() in
+      assume(MonotoneMap.fresh (secret_ideal k) x h); // FIXME(adl)!!
+      MonotoneMap.extend (secret_ideal k) x dk;
+      (| i', dk |)
+  else
     let raw =
-      HKDF.expand #(a.ha) k (Platform.Bytes.abytes lbl) (UInt32.v (use.pkg'.len a')) in 
-    assume(honest i' ==> honest i); //17-10-31 TODO with Antoine
-    use.pkg'.coerce i' a' raw
+      HKDF.expand #(a.ha) (secret_corrupt k) (Platform.Bytes.abytes lbl) (UInt32.v (use.pkg'.len a')) in
+    let dk = use.pkg'.coerce i' a' raw in
+    (| i', dk |)
 
 /// Outlining a global KDF state invariant, supported by package
 /// definition tables for all derivable functionalities.
@@ -527,11 +719,11 @@ let derive #u #i a k lbl ctx =
 ///   let i' = Derive lbl ctx in
 ///   wellformed_id i' ==>
 ///   let u = u_of_i i in
-///   let pkg',... = u lbl in 
+///   let pkg',... = u lbl in
 ///   match KDF.lookup i with
 ///   | None -> None? pkg'.lookup i' // used when creating PRFs
 ///   | Some k -> pkg'.lookup i' == lookup k (Domain lbl ctx) // used when extending PRFs.
-/// 
+///
 /// The invariant is restored by the time derive return.
 /// (note we implicitly rely on u_of_i)
 
@@ -541,59 +733,83 @@ let derive #u #i a k lbl ctx =
 
 /// key-derivation table (memoizing create/coerce)
 
-val ssa: #a:Type0 -> Preorder.preorder (option a) 
-let ssa #a = 
-  let f x y = 
-    match x,y with 
-    | None, _  -> True 
-    | Some v, Some v' -> v == v'
-    | _ -> False in
-  f
+assume val ssa: #a:Type0 -> Preorder.preorder (option a)
+
+assume val flag_KEF0: b:bool{b ==> model /\ flag_KDF ==> b}
+type idealKEF0 = b2t flag_KEF0
+assume val lemma_kdf_kef0: unit -> Lemma (idealKDF ==> idealKEF0)
+
+let safeKEF0 (i:regid) = idealKEF0 /\ honest i
+let corruptKEF0 (i:regid) = idealKEF0 ==> corrupt i
 
 // memoizing a single extracted secret
-private type mref_secret (u: usage info) (i: id) = 
-  // would prefer: HyperStack.mref (option (secret u i)) (ssa #(secret u i))
-  Monotonic.RRef.m_rref there (option (secret u i)) ssa
+private type mref_secret (u: usage info) (i: regid) =
+  MR.m_rref there (option (secret u i)) ssa
 
 /// covering two cases: application PSK and resumption PSK
 /// (the distinction follow from the value of i)
-type psk (u: usage info) (i: id) = (
-  let i' = Derive i "" Extract in 
-  if (* Flags.extract0 && *) honest i 
-  then mref_secret u i'
-  else lbytes (secret_len (get_info i')))
+type psk (u: usage info) (i: regid) =
+  ir_key safeKEF0 (mref_secret u i) (real_secret i) i
 
-let mref_secret_psk (u: usage info) (i: id) (s:mref_secret u (Derive i "" Extract){honest i}) : psk u i = s
-let psk_mref_secret (#u: usage info) (#i: id) (p:psk u i{honest i}) : mref_secret u (Derive i "" Extract) = p
+let psk_ideal (#u: usage info) (#i:regid) (p:psk u i {safeKEF0 i}): mref_secret u i =
+  let t : s:ideal_or_real (mref_secret u i) (real_secret i) {safeKEF0 i <==> Ideal? s} = p in
+  Ideal?.v t
 
-val coerce_psk: 
+let ideal_psk (#u: usage info) (#i:regid) (t: mref_secret u i{safeKEF0 i}) : psk u i =
+  let t : s:ideal_or_real (mref_secret u i) (real_secret i) {safeKEF0 i <==> Ideal? s} = Ideal t in
+  assert(model); t
+
+let psk_real (#u: usage info) (#i:regid) (p:psk u i {corruptKEF0 i}): real_secret i =
+  lemma_honest_corrupt i;
+  if model then
+    let t : s:ideal_or_real (mref_secret u i) (real_secret i) {safeKEF0 i <==> Ideal? s} = p in
+    Real?.v t
+  else p
+
+let real_psk (#u: usage info) (#i:regid) (t: real_secret i{corruptKEF0 i}) : psk u i =
+  if model then
+    (lemma_honest_corrupt i;
+    let s : s:ideal_or_real (mref_secret u i) (real_secret i) {safeKEF0 i <==> Ideal? s} = Real t in s)
+  else t
+
+type ext0 (u:usage info) (i:regid) =
+  i':regid{i' == Derive i "" Extract} & psk u i'
+
+val coerce_psk:
   #u: usage info ->
-  i: id -> 
-  a: info {a == get_info i} -> 
-  raw: lbytes (secret_len a) -> 
-  ST (psk u i)
-  (requires fun h0 -> ~(honest i))
+  i: regid ->
+  a: info {a == get_info i} ->
+  raw: lbytes (secret_len a) ->
+  ST (ext0 u i)
+  (requires fun h0 -> idealKEF0 ==> corrupt i)
   (ensures fun h0 p h1 -> (*TBC*) True)
-let coerce_psk #u i a raw = raw
 
-val create_psk: 
+let coerce_psk #u i a raw =
+  let i', honest' = register_derive i "" Extract in
+  lemma_corrupt_invariant i "" Extract;
+  (| i', real_psk #u #i' raw |)
+
+val create_psk:
   #u: usage info ->
-  i: id -> 
-  a: info {a == get_info i} -> 
-  ST (psk u i)
+  i: regid ->
+  a: info {a == get_info i} ->
+  ST (ext0 u i)
   (requires fun h0 -> True)
   (ensures fun h0 p h1 -> (*TBC*) True)
-let create_psk #u i a = 
-  if honest i then 
-    let i': id = Derive i "" Extract in 
-    let t' = secret u i' in 
-    mref_secret_psk u i (Monotonic.RRef.m_alloc there None) // better style or library call? 
-  else 
-    coerce_psk #u i a (sample (secret_len a)) 
+let create_psk #u i a =
+  let i', honest' = register_derive i "" Extract in
+  lemma_corrupt_invariant i "" Extract;
+  if flag_KEF0 && honest' then
+    let t' = secret u i' in
+    let r: mref_secret u i' = MR.m_alloc #(option t') #(ssa #t') there None in
+    (| i', ideal_psk #u #i' r |)
+  else
+    (| i', real_psk #u #i' (sample (secret_len a)) |)
 
-let pskp (*ip:ipkg*) (u:usage info): pkg info (ii get_info) = Pkg 
-  (psk u)
+let pskp (*ip:ipkg*) (u:usage info): pkg info (ii get_info) = Pkg
+  (ext0 u)
   secret_len
+  idealKEF0
   create_psk
   coerce_psk
 
@@ -601,129 +817,149 @@ let pskp (*ip:ipkg*) (u:usage info): pkg info (ii get_info) = Pkg
 /// possibly customized on the distribution of k.
 val extract0:
   #u: usage info ->
-  #i: id ->
-  k: psk u i -> 
+  #i: regid ->
+  k: ext0 u i ->
   a: info {a == get_info i} ->
-  ST 
-    (secret u (Derive i "" Extract))
+  ST
+    (secret u (dfst k))
     (requires fun h0 -> True)
     (ensures fun h0 p h1 -> (*TBC*) True)
 
-let extract0 #u #i k a = 
-  let i': id = Derive i "" Extract in 
-  if (* Flags.extract0 && *) honest i 
-  then 
-    match Monotonic.RRef.m_read (psk_mref_secret k) with 
+let extract0 #u #i k a =
+  let (| i', p |) = k in
+  let honest' = get_honest i' in
+  lemma_kdf_kef0 (); // idealKDF ==> idealKEF0
+  if flag_KEF0 && honest'
+  then
+    let k: mref_secret u i' = psk_ideal p in
+    match MR.m_read k with
     | Some extract -> extract
-    | None -> 
-        let extract = create u i' a in 
-        assume false; //TODO framing the empty mref
-        Monotonic.RRef.m_write (psk_mref_secret k) (Some extract); 
-        extract 
-  else 
-    let raw = HKDF.extract #(a.ha) (Hashing.zeroHash a.ha) k in 
-    assume(honest i' ==> honest i); //17-10-31 TODO with Antoine
+    | None ->
+      let extract = create u i' a in
+      let mrel = ssa #(secret u i') in
+      let () =
+        MR.m_recall k;
+        let h = get() in
+        assume (MR.m_sel h k == None); // TODO framing of call to create
+        assume (mrel None (Some extract)); // TODO Fix the monotonic relation
+        MR.m_write k (Some extract) in
+      extract
+  else
+    let k = psk_real p in
+    let raw = HKDF.extract #(a.ha) (Hashing.zeroHash a.ha) k in
     coerce u i' a raw
-
 
 /// The "salt" is an optional secret used (exclusively) as HKDF
 /// extraction key. The absence of salt (e.g. when no PSK is used) is
 /// handled using a special, constant salt marked as compromised.
-/// 
+///
 /// salt is indexed by the usage of the secret that will be extracted
 /// (the usage of the salt itself is fixed).
 ///
 /// We use separate code for salt1 and salt2 because they are
 /// separately idealized (salt1 is more complicated)
 
+assume val flag_PRF1: b:bool{flag_KDF ==> b /\ b ==> model /\ flag_KEF0 ==> b}
+let idealPRF1 = b2t flag_PRF1
+let lemma_kdf_prf1 () : Lemma (idealKDF ==> idealPRF1) = admit()
+
+type safePRF1 (i:regid) = idealPRF1 /\ honest i
+type corruptPRF1 (i:regid) = idealPRF1 ==> corrupt i
+
 assume type salt (u: usage info) (i: id)
 
-assume val create_salt: 
-  #u: usage info -> 
-  i: id -> 
-  a: info -> 
-  salt u i
-
-assume val coerce_salt: 
+assume val create_salt:
   #u: usage info ->
   i: id ->
-  a: info -> 
-  raw: lbytes (secret_len a) ->
-  salt u i 
+  a: info ->
+  salt u i
 
-let saltp (*ip:ipkg*) (u:usage info): pkg info (ii get_info) = Pkg 
+assume val coerce_salt:
+  #u: usage info ->
+  i: id ->
+  a: info ->
+  raw: lbytes (secret_len a) ->
+  salt u i
+
+let saltp (*ip:ipkg*) (u:usage info): pkg info (ii get_info) = Pkg
   (salt u)
   secret_len
-  create_salt 
+  idealPRF1
+  create_salt
   coerce_salt
-
 
 /// HKDF.Extract(key=s, materials=dh_secret) idealized as 2-step
 /// (KEF-ODH, KEF-Salt game); we will need separate calls for clients
 /// and servers.
 
 /// two flags; we will idealize ODH first
-/// 
-assume val flag_prf1: bool 
-assume val flag_odh: b:bool { (flag_prf1 ==> b) /\ (b ==> Flags.ideal_KEF) } 
+assume val flag_ODH: b:bool { (flag_PRF1 ==> b) /\ (b ==> model)}
+type idealODH = b2t flag_ODH
+
+type safeODH (i:regid) = idealODH /\ honest i
+type corruptODH (i:regid) = idealODH ==> corrupt i
 
 /// we write prf_ for the middle salt-keyed extraction, conditionally
 /// idealized as a PRF keyed by salt1 depending on flag_prf1
-/// 
+///
 /// its interface provides create, coerce, leak, and extract its
 /// internal table memoizes it either with *wide* domain gZ, or with
 /// *narrow* domain idh
 ///
-/// Returns a narrow-indexed key, 
-/// 
+/// Returns a narrow-indexed key,
+///
 /// its internal state ensures sharing
 ///
 assume val prf_leak:
-  #u: usage info -> 
-  #i: id ->
-  #a: info {a == get_info i} -> //NS: why do you needs this parameter? It can only be inferred in a brittle way using the syntactic shape of the result type; and it also seems redundant since it can be computed from i. CF: the intent is that [i] (with all provenance details) will be erased, whereas [a] (with what we need at runtime) will be checked against i then extracted. We could make [a] explicit in all such functions (we currently use both styles).
-  s: salt u i { flag_prf1 ==> ~(honest i)} -> Hashing.Spec.hkey a.ha
-// revisit flag condition, a bit awkward.
+  #u: usage info ->
+  #i: regid ->
+  #a: info {a == get_info i} ->
+  s: salt u i {idealPRF1 ==> corrupt i} ->
+  Hashing.Spec.hkey a.ha
+
+type ext1 (u:usage info) (i:regid) (idh:id_dhe) =
+  i':regid{i' == Derive i "" (ExtractDH idh)} & secret u i'
 
 val prf_extract1:
-  #u: usage info -> 
-  #i: id ->
-  a: info {a == get_info i} -> 
+  #u: usage info ->
+  #i: regid ->
+  a: info {a == get_info i} ->
   s: salt u i ->
-  idh: id_dhe ->
-  gZ: bytes -> 
-  ST (secret u (Derive i "" (ExtractDH idh)))
-  (requires fun h0 -> True) 
+  idh: id_dhe{~(honest_idh (ExtractDH idh))} ->
+  gZ: bytes ->
+  ST (ext1 u i idh)
+  (requires fun h0 -> True)
   (ensures fun h0 k h1 -> True)
 
-let prf_extract1 #u #i a s idh gZ = 
-  let j: id = Derive i "" (ExtractDH idh) in
-  if flag_prf1 && honest i 
-  then 
+let prf_extract1 #u #i a s idh gZ =
+  let j, honest' = register_derive i "" (ExtractDH idh) in
+  lemma_corrupt_invariant i "" (ExtractDH idh);
+  let honest = get_honest i in
+  lemma_kdf_prf1 ();
+  if flag_PRF1 && honest
+  then
     (* TBD: memoization
-    let w = 
+    let w =
       // "wide" PRF, memoized on gZ
-      match find s.wide gZ with 
+      match find s.wide gZ with
       | Some w -> w // may return k
-      | None -> 
+      | None ->
         let w = pkg.create0 j a in
         s.wide := snoc s.wide w;
         w in  *)
-    create u j a 
+    (| j, create u j a |)
     // agreement on the algorithms follows from the salt.
-  else 
-    let raw_salt = prf_leak #u #i #a s in 
-    let raw = HKDF.extract raw_salt  gZ (* narrow, concrete *) in 
-    assume (~(honest j));
-    coerce u j a raw 
-
+  else
+    let raw_salt = prf_leak #u #i #a s in
+    let raw = HKDF.extract raw_salt gZ (* narrow, concrete *) in
+    (| j, coerce u j a raw |)
 
 /// ODH (precisely tracking the games, not yet code-complete
 /// --------------------------------------------------------------------------------------------------
 
 // Ideally, we maintain a monotonic map from every honestly-sampled
 // initiator share gX to its set of honestly-sampled responders shares
-// (i,gY). 
+// (i,gY).
 // The table exists when [Flags.ideal_KDF], a precondition for [flag_odh]
 
 // We need a variant of MonotoneMap that enables monotonic updates to
@@ -737,95 +973,93 @@ let prf_extract1 #u #i a s idh gZ =
 // should be entirely static. Intuitively, there is a function from
 // indexes to usage. Probably definable with the actual usage (big
 // mutual reduction?)
-assume val u_of_i: i:id -> usage info 
+assume val u_of_i: i:id -> usage info
 
-let peer_table (#g: CommonDH.group) (gX: CommonDH.share g): Type0 = 
-  MonotoneMap.t there 
-    (i:id * gY: CommonDH.share g)
-    (fun i_gY -> 
-      let (i, gY) = i_gY in 
-      secret (u_of_i i) (Derive i "" (ExtractDH (IDH gX gY))))
-    (fun _ -> True)
+type odhid = x:CommonDH.dhi{CommonDH.registered_dhi x}
 
-let odh_table = 
-  MonotoneMap.t there 
-  (g: CommonDH.group & gX: CommonDH.share g)
-  (fun (| g, gX |) -> _: peer_table gX{CommonDH.honest_share (|g, gX|)})
-  (fun _ -> True)
+type peer_index (x:odhid) =
+  i:regid & y:CommonDH.dhr x {CommonDH.registered_dhr y /\ registered (Derive i "" (ExtractDH (IDH x y)))}
 
-let odh_state: (if Flags.ideal_KEF then odh_table else unit) = 
-  if Flags.ideal_KEF
-  then alloc () <: odh_table // 17-11-04 convenient use of subtyping
+type peer_instance (#x:odhid) (iy:peer_index x) =
+  secret (u_of_i (dfst iy)) (Derive (dfst iy) "" (ExtractDH (IDH x (dsnd iy))))
+
+let peer_table (x:odhid): Type0 =
+  MM.t there (peer_index x) (peer_instance #x) (fun _ -> True)
+type odh_table = MM.t there odhid peer_table (fun _ -> True)
+
+let odh_state : (if model then odh_table else unit) =
+  if model then MM.alloc #there #odhid #peer_table #(fun _ -> True)
   else ()
 
-val honest_gX: #g:CommonDH.group -> gX: CommonDH.share g -> Type0 
-let honest_gX #g gX = 
-  if Flags.ideal_KEF then 
-    let t: odh_table = odh_state in 
-    Monotonic.RRef.witnessed (MonotoneMap.defined t (|g,gX|))
-  else True
-//17-10-22 why can't I write flag_odh ==> ... ? {logic} error   
-//17-10-23 for now we could use that style only with an annotated let instead of val;let
+type odh_fresh (i:odhid) (h:mem) =
+  (if model then
+    let log : odh_table = odh_state in
+    MM.fresh log i h
+  else True)
 
-val test_honest_gX: #g:CommonDH.group -> gX: CommonDH.share g -> ST (b:bool)
-  (requires fun h0 -> Flags.ideal_KEF)
-  (ensures fun h0 b h1 -> 
-    h0 == h1 /\ 
-    Flags.ideal_KEF /\ 
-    (let t: odh_table = odh_state in 
-    ( b2t b == MonotoneMap.defined t (|g,gX|) h1) /\
-      (b ==> honest_gX gX)
-    ))
-let test_honest_gX #g gX = 
-  let t: odh_table = odh_state in
-  match MonotoneMap.lookup t (|g,gX|) with
-  | Some _ -> true
-  | None -> false
+let lemma_fresh_odh (i:CommonDH.dhi) (h:mem)
+  : Lemma (CommonDH.fresh_dhi i h ==> odh_fresh i h)
+  = admit () // i:dhi implies registered_dhi i and registered_dhi i /\ fresh_dhi i h ==> False
 
+let lemma_fresh_odh_framing (i:CommonDH.dhi) (h0:mem) (h1:mem)
+  : Lemma (odh_fresh i h0 /\ modifies_one CommonDH.dh_region h0 h1 ==> odh_fresh i h1)
+  = admit() // assume(HH.disjoint there CommonDH.dh_region)
 
-//assume val info_id: i:id -> a: info
+type odh_defined (i:odhid) =
+  (if model then
+    let log : odh_table = odh_state in
+    MR.witnessed (MM.defined log i)
+  else True)
 
+type odhr_fresh (#i:odhid) (r:peer_index i) (h:mem) =
+  (if model then
+    let log : odh_table = odh_state in
+    (match MM.sel (MR.m_sel h log) i with
+    | Some t ->
+      (match MM.sel (MR.m_sel h t) r with
+      | None -> True
+      | _ -> False)
+    | _ -> False)
+  else True)
 
-#set-options "--print_universes --print_implicits"
+let lemma_fresh_dhr (#i:odhid) (r:peer_index i) (h:mem)
+  : Lemma (CommonDH.fresh_dhr (dsnd r) h ==> odhr_fresh r h)
+  = admit () // contradition on  CommonDH.registered_dhr y
 
-// assume val peer_gX: #g:CommonDH.group -> i:id -> gX: CommonDH.share g -> gY: CommonDH.share g {wellformed_id (Derive i "" (ExtractDH (Some (| g, gX, gY |))))} -> 
-//   option (secret 
-//     (u_of_i i)
-//     (Derive i "" (ExtractDH (Some (| g, gX, gY |)))) 
-//     (info_id (Derive i "" (ExtractDH (Some (| g, gX, gY |))))))
-
-
-// let peers_gX #g gx = let t: peer_table = odh_table in MonotoneMap.lookup h0.[t] (|g,gX|)
-
-// ideal state 
-// val peer: mref (map gX --> list (i,gY)) 
-// - presence codes I[X]
-// - contents codes R[X] 
-// conversely [keyshare] locally provides  x
+let lemma_fresh_dhr_framing (#i:odhid) (r:peer_index i) (h0:mem) (h1:mem)
+  : Lemma (odhr_fresh r h0 /\ modifies (Set.union (Set.singleton CommonDH.dh_region) (Set.singleton honest_region)) h0 h1 ==> odhr_fresh r h1)
+  = admit() // assume(HH.disjoint there CommonDH.dh_region)
 
 /// Client-side instance creation
 /// (possibly used by many honest servers)
-val odh_init: g: CommonDH.group -> ST (CommonDH.keyshare g)
+val odh_init: g: CommonDH.group -> ST (CommonDH.ikeyshare g)
   (requires fun h0 -> True)
-  (ensures fun h0 x h1 -> honest_gX (CommonDH.pubshare x))
-// TODO framing: we only modify the global table regions for CommonDH and ODH
- 
-let odh_init g = 
-  let x = CommonDH.keygen g in 
-  if Flags.ideal_KEF then (
-    let t: odh_table = odh_state in 
-    let gX: CommonDH.share g = CommonDH.pubshare x in  
-    assert(CommonDH.honest_share (|g,gX|));
-    // TODO 17-10-22 since gX is freshly registered, we statically
-    // know it can't occur in the peers table; what's a better keygen
-    // spec for that?
-    let peers = alloc  () <: peer_table gX in
-    if None? (MonotoneMap.lookup t (|g,gX|)) then MonotoneMap.extend t (|g,gX|) peers;
-    assert(honest_gX gX)
-    );
-  x // could additionally return gX 
-// TODO crypto agility: do we record keygen as honest for a bad group? 
+  (ensures fun h0 x h1 ->
+    let gx : CommonDH.dhi = (| g, CommonDH.ipubshare x |) in
+    modifies (Set.union (Set.singleton CommonDH.dh_region) (Set.singleton there)) h0 h1
+    /\ model ==> (odh_fresh gx h0 /\ odh_defined gx /\ CommonDH.honest_dhi gx))
 
+let odh_init g =
+  let h0 = get () in
+  let x = CommonDH.keygen g in
+  let h1 = get () in
+  if model then
+   begin
+    let log : odh_table = odh_state in
+    let i : CommonDH.dhi = (| g, CommonDH.ipubshare x |) in
+    lemma_fresh_odh i h0;
+    lemma_fresh_odh_framing i h0 h1;
+    assert(MM.sel (MR.m_sel h1 log) i == None);
+    let peers : peer_table i = MM.alloc #there #(peer_index i) #(peer_instance #i) #(fun _ -> True) in
+    let h2 = get () in
+    assume(MM.sel (MR.m_sel h2 log) i == None); // FIXME allocate peers somewhere else !!
+    MM.extend log i peers;
+    assume(MR.stable_on_t log (MM.defined log i));
+    MR.witness log (MM.defined log i)
+   end;
+  x
+
+// TODO crypto agility: do we record keygen as honest for a bad group?
 
 /// Server-side creation and completion
 ///
@@ -835,84 +1069,106 @@ let odh_init g =
 ///
 /// We require that gX be the share of a honest initiator,
 /// but not that they agree on the salt index
+
+private let register_odh (i:regid) (gX:CommonDH.dhi) (gY:CommonDH.dhr gX)
+  : ST (j:regid{j == Derive i "" (ExtractDH (IDH gX gY))})
+  (requires fun h0 -> model /\ CommonDH.honest_dhr gY)
+  (ensures fun h0 _ h1 -> modifies_one honest_region h0 h1)
+  =
+  let idh = IDH gX gY in
+  let ctx = ExtractDH idh in
+  assert(honest_idh ctx);
+  let j = Derive i "" ctx in // N.B. this is the only case where i can be corrupt and j honest
+  let hlog : i_honesty_table = honesty_table in
+  MR.m_recall hlog;
+  match MM.lookup hlog j with
+  | None ->
+    let m = MR.m_read hlog in
+    assume(honesty_invariant (MM.upd m j true)); // Sepcial case: honest IDH
+    MM.extend hlog j true;
+    MM.contains_stable hlog j true;
+    MR.witness hlog (MM.contains hlog j true); j
+  | Some b -> j
+
 val odh_test:
-  #u: usage info -> 
-  #i: id -> 
-  a: info {a == get_info i} ->  //NS: Again, why this parameter that can be computed from i?
+  #u: usage info ->
+  #i: regid ->
+  a: info {a == get_info i} ->
   s: salt u i ->
-  g: CommonDH.group ->
-  gX: CommonDH.share g -> 
-  ST ( 
-    gY:CommonDH.share g &
-    secret u (Derive i "" (ExtractDH (IDH gX gY))))
-  (requires fun h0 -> honest_gX gX)
-  (ensures fun h0 r h1 -> 
+  gX: odhid{odh_defined gX} ->
+  ST (j:peer_index gX{dfst j == i} & peer_instance j)
+  (requires fun h0 -> model /\ CommonDH.honest_dhi gX)
+  (ensures fun h0 r h1 ->
     // todo, as sanity check
-    // let (|gY, s|) = dfst r in 
+    // let (|gY, s|) = dfst r in
     // flag_odh ==> s == peer_gX gY
     True)
 
-let odh_test #u #i a s g gX = 
+let odh_test #u #i a s gX =
   assume (u == u_of_i i); //17-11-01 TODO modelling
   (* we get the same code as in the game by unfolding dh_responder, e.g.
-  let y = CommonDH.keygen g in 
-  let gY = CommonDH.pubshare y in  
+  let y = CommonDH.keygen g in
+  let gY = CommonDH.pubshare y in
   let gZ: bytes (*CommonDH.share g*) = ... in  // used only when (not flag_odh)
   *)
-  let gY, gZ = CommonDH.dh_responder gX in 
-  let idh = IDH gX gY in
-  let j = Derive i "" (ExtractDH idh) in 
+  let h0 = get() in
+  let gY, gZ = CommonDH.dh_responder (dfst gX) (dsnd gX) in
+  let j = register_odh i gX gY in
+  let j' : peer_index gX = (| i, gY |) in
+  let h1 = get() in
+  lemma_fresh_dhr j' h0;
+  lemma_fresh_dhr_framing j' h0 h1;
+  assert(odhr_fresh j' h1);
   assert(a == get_info j);
-  let k: secret u j = 
-    if flag_odh
-    then (*KDF.*) create u j a (* narrow *)
-    else 
-      // we know the salt is dishonest because flag_kdf is off
-      let raw = HKDF.extract #a.ha (prf_leak s) gZ (* wide, concrete *) in 
-      //TODO deduce that j is dishonest too.
-      assume(~(honest j));
-      coerce u j a raw in
-  if Flags.ideal_KEF then (
-      let t: odh_table = odh_state in 
-      // guaranteed to succeed by honest_gX 
-      Monotonic.RRef.testify(MonotoneMap.defined t (|g,gX|));
-      let peers = Some?.v (MonotoneMap.lookup t (|g,gX|)) in 
-      if None? (MonotoneMap.lookup peers (i,gY)) then 
-      MonotoneMap.extend peers (i,gY) k
-      );
-  (| gY, k |) 
+  let k: secret u j =
+    if flag_ODH then create u j a (* narrow *)
+    else (
+      assert(~idealPRF1);
+      let raw = HKDF.extract #a.ha (prf_leak s) gZ (* wide, concrete *) in
+      assume(~idealKDF); // FIXME(adl): fix the loop in the flag order dependency. See definition of usage for proposed solution
+      coerce u j a raw
+    ) in
+  let h2 = get() in
+  assume(odhr_fresh j' h2); // TODO framing of KDF
+  let t: odh_table = odh_state in
+  MR.testify(MM.defined t gX);
+  let peers = Some?.v (MM.lookup t gX) in
+  MM.extend peers j' k;
+  (| j' , k |)
+
+unfold let idh_of (#g:CommonDH.group) (x:CommonDH.ikeyshare g) (gY:CommonDH.rshare g (CommonDH.ipubshare x)) =
+  IDH (| g, CommonDH.ipubshare x |) gY
 
 // the PRF-ODH oracle, computing with secret exponent x
 val odh_prf:
-  #u: usage info -> 
-  #i: id -> 
-  a: info {a == get_info i}->  //NS: idem
+  #u: usage info ->
+  #i: regid ->
+  a: info {a == get_info i}->
   s: salt u i ->
   g: CommonDH.group ->
-  x: CommonDH.keyshare g -> 
-  gY: CommonDH.share g -> 
-  ST (
-    let gX = CommonDH.pubshare x in 
-    let idh = IDH gX gY in //17-10-31 BUG? adding the eta-expansion was necessary
-    secret u (Derive i "" (ExtractDH idh)))
-    (requires fun h0 -> 
-      let gX = CommonDH.pubshare x in
-      honest_gX gX /\ (
-      Flags.ideal_KEF ==> (
-        let t: odh_table = odh_state in  //NS: This coercion is a necessary, common pattern. CF: when to use an auxiliary function vs an auxiliary let?
-        MonotoneMap.defined t (|g,gX|) h0 /\ (
-        let peers = MonotoneMap.value t (|g,gX|) h0 in 
-        ~ (MonotoneMap.defined peers (i,gY) h0)))))  // what a mouthful NS: aside from the coercion above which I don't see how to remove easily, compressing this post-condition seems to be an application-specific thing, right? i.e, you could define some abbreviation to stand for this predicate
-    (ensures fun h0 _ h1 -> True)
+  x: CommonDH.ikeyshare g ->
+  gY: CommonDH.rshare g (CommonDH.ipubshare x) ->
+  ST (i':regid{i' == Derive i "" (ExtractDH (idh_of x gY))} & secret u i')
+  (requires fun h0 ->
+    let gX : CommonDH.dhi = (| g, CommonDH.ipubshare x |) in
+    CommonDH.honest_dhi gX /\ odh_defined gX
+    /\ (model ==> (CommonDH.fresh_dhr #gX gY h0)))
+  (ensures fun h0 _ h1 -> True)
 
-// requires peer[gX] is defined (witnessed in x) and does not contain (i,gY)
-// None? (find (i, gY) !peer[gX])
-let odh_prf #u #i a s g x gY = 
-  let gX = CommonDH.pubshare x in 
+// FIXME. Lemma is false. Not sure how to fix
+let lemma_fresh_dhr_hinv (#x:CommonDH.dhi) (y:CommonDH.dhr x) (h:mem)
+  : Lemma (requires (model ==> CommonDH.fresh_dhr #x y h))
+          (ensures ~(honest_idh (ExtractDH (IDH x y))))
+  = admit()
+
+let odh_prf #u #i a s g x gY =
+  let h = get () in
+  let gX : CommonDH.dhi = (| g, CommonDH.ipubshare x |) in
   let idh = IDH gX gY in
-  let gZ = CommonDH.dh_initiator x gY in
-  prf_extract1 a s idh gZ
-
+  lemma_fresh_dhr_hinv #gX gY h;
+  let gZ = CommonDH.dh_initiator g x gY in
+  let (| i', s |) = prf_extract1 a s idh gZ in
+  (| i', s |)
 
 /// --------------------------------------------------------------------------------------------------
 /// Diffie-Hellman shares
@@ -922,153 +1178,216 @@ let odh_prf #u #i a s g x gY =
 // [abstract type private_keyshare g = mref bool ...] that enables
 // calling it exactly once
 
-/// Initiator computes DH keyshare, irrespective of the KDF & salt. 
-let initI (g:CommonDH.group) = odh_init g 
+/// Initiator computes DH keyshare, irrespective of the KDF & salt.
+let initI (g:CommonDH.group) = odh_init g
 
 /// Responder computes DH secret material
 val extractR:
-  #u: usage info -> 
-  #i: id -> 
+  #u: usage info ->
+  #i: regid ->
   s: salt u i ->
-  a: info {a == get_info i} -> 
-  g: CommonDH.group ->
-  gX: CommonDH.share g ->
-  ST( 
-    gY:CommonDH.share g & (
-      secret u (Derive i "" (ExtractDH (IDH gX gY)))))
-    (requires fun h0 -> True)
-    (ensures fun h0 _ h1 -> True)
-let extractR #u #i s a g gX = 
-  let b = 
-    if Flags.ideal_KEF then test_honest_gX gX else false in
-  if b 
-  then odh_test a s g gX
+  a: info {a == get_info i} ->
+  gX: odhid ->
+  ST(i_gY:peer_index gX{dfst i_gY == i} & peer_instance i_gY)
+  (requires fun h0 -> True)
+  (ensures fun h0 _ h1 -> True)
+
+let extractR #u #i s a gX =
+  let b = if model then CommonDH.is_honest_dhi gX else false in
+  if b then
+   begin
+    let t: odh_table = odh_state in
+    (if None? (MM.lookup t gX) then
+      let peers = MM.alloc #there #(peer_index gX) #(peer_instance #gX) #(fun _ -> True) in
+      let h = get() in
+      assume(None? (MM.sel (MR.m_sel h t) gX));
+      MM.extend t gX peers;
+      assume(MR.stable_on_t t (MM.defined t gX));
+      MR.witness t (MM.defined t gX));
+    odh_test a s gX
+   end
   else
+   begin
     // real computation: gY is honestly-generated but the exchange is doomed
-    let gY, gZ = CommonDH.dh_responder gX in 
+    let gY, gZ = CommonDH.dh_responder (dfst gX) (dsnd gX) in
     let idh = IDH gX gY in
-    let j = Derive i "" (ExtractDH idh) in 
-    let k = prf_extract1 a s idh gZ in
-    (| gY, k |)
+    assume(~(honest_idh (ExtractDH idh))); // FIXME
+    let (| i', k |) : ext1 u i idh = prf_extract1 a s idh gZ in
+    assert(i' == Derive i "" (ExtractDH idh));
+    let k : secret u (Derive i "" (ExtractDH idh)) = k in
+    let i_gY : peer_index gX = (| i, gY |) in
+    let s : peer_instance #gX i_gY = admit() in
+    (| i_gY, s |)
+   end
+
+(*)
+     let gX : CommonDH.dhi = (| g, CommonDH.ipubshare x |) in
+     CommonDH.honest_dhi gX /\ odh_defined gX
+     /\ (model ==> (CommonDH.fresh_dhr #gX gY h0)))
+*)
 
 /// Initiator computes DH secret material
-val extractI: 
-  #u: usage info -> 
-  #i: id -> 
+val extractI:
+  #u: usage info ->
+  #i: regid ->
   a: info {a == get_info i} ->
   s: salt u i ->
   g: CommonDH.group ->
-  x: CommonDH.keyshare g ->
-  gY: CommonDH.share g ->
-  ST(secret u (Derive i "" (ExtractDH (IDH (CommonDH.pubshare x) gY))))
-  (requires fun h0 -> honest_gX (CommonDH.pubshare x))
+  x: CommonDH.ikeyshare g ->
+  gY: CommonDH.rshare g (CommonDH.ipubshare x) ->
+  ST(i':regid{i' == Derive i "" (ExtractDH (idh_of x gY))} & secret u i')
+  (requires fun h0 ->
+    let gX : CommonDH.dhi = (| g, CommonDH.ipubshare x |) in
+    CommonDH.honest_dhi gX /\ odh_defined gX)
   (ensures fun h0 k h1 -> True)
 
-let extractI #u #i a s g x gY = 
-  if Flags.ideal_KEF then 
-    let gX = CommonDH.pubshare x in
-    let t: odh_table = odh_state in 
-    Monotonic.RRef.testify(MonotoneMap.defined t (|g,gX|));
-    let idh = IDH (CommonDH.pubshare x) gY in
-    let peers = Some?.v (MonotoneMap.lookup t (|g,gX|)) in 
+let extractI #u #i a s g x gY =
+  let gX : CommonDH.dhi = (| g, CommonDH.ipubshare x |) in
+  let b = if model then CommonDH.is_honest_dhi gX else false in
+  if b then
+    let t: odh_table = odh_state in
+    MR.testify(MM.defined t gX);
+    let peers = Some?.v (MM.lookup t gX) in
+    let idh = IDH gX gY in
     let i' = Derive i "" (ExtractDH idh) in
+    assume(registered i');
     assert(wellformed_id i);
-    assert(wellformed_id i');
+    assume(wellformed_id i'); //17-11-01 same as above?
+    let i_gY : peer_index gX = (| i, gY |) in
     let ot = secret u i' in
     assume (u == u_of_i i); //17-11-01 indexing does not cover u yet
-    let o : option ot = MonotoneMap.lookup peers (i,gY) in
-    match o with 
-    | Some k -> k
-    | None -> odh_prf #u #i a s g x gY
+    let o : option ot = MM.lookup peers i_gY in
+    match o with
+    | Some k -> (| i', k |)
+    | None -> assume false; odh_prf #u #i a s g x gY
   else odh_prf #u #i a s g x gY
 
-val extractP: 
+val extractP:
   #u:usage info ->
-  #i: id ->
-  a: info {a == get_info i} -> 
+  #i: regid ->
+  a: info {a == get_info i} ->
   s: salt u i ->
-  ST(secret u (Derive i "" (ExtractDH NoIDH)))
+  ST(i':regid{i' == Derive i "" (ExtractDH NoIDH)} & secret u i')
   (requires fun h0 -> True)
   (ensures fun h0 r h1 -> True)
-let extractP #u #i a s = 
+let extractP #u #i a s =
   let gZ = Hashing.Spec.zeroHash a.ha in
-  prf_extract1 a s NoIDH gZ
+///17-11-01 stuck on this one too.
+  admit()
+  // prf_extract1 a s NoDHE gZ
 
+assume val flag_KEF2: b:bool{flag_KDF ==> b}
+type idealKEF2 = b2t flag_KEF2
+
+type safeKEF2 i = idealKEF2 /\ honest i
+type corruptKEF2 i = idealKEF2 ==> corrupt i
 
 /// ---------------- final (useless) extraction --------------------
-/// 
-type salt2 (u: usage info) (i: id) = (
-  let i' = Derive i "" Extract in 
-  if (*TODO Flags.ideal && *) honest i  
-  then mref_secret u i'
-  else lbytes (secret_len (get_info i')))
+///
+type salt2 (u: usage info) (i:regid) =
+  ir_key safeKEF2 (mref_secret u i) (real_secret i) i
 
 // same code as for PSKs; but extract0 and extract2 differ concretely
 
-val coerce_salt2: 
-  #u: usage info ->
-  i: id ->
-  a: info {a == get_info i} -> 
-  raw: lbytes (secret_len a) ->
-  ST (salt2 u i)
-  (requires fun h0 -> ~(honest i))
-  (ensures fun h0 p h1 -> (*TBC*) True)
-let coerce_salt2 #u i a raw = raw
+let real_salt2 (#u: usage info) (#i:regid) (t: real_secret i{corruptKEF2 i}) : salt2 u i =
+  if model then
+    (lemma_honest_corrupt i;
+    let s : s:ideal_or_real (mref_secret u i) (real_secret i) {safeKEF2 i <==> Ideal? s} = Real t in s)
+  else t
 
-val create_salt2: 
-  #u: usage info -> 
-  i: id -> 
-  a: info {a == get_info i} -> 
-  ST (salt2 u i)
+let salt2_real (#u: usage info) (#i:regid) (p:salt2 u i {corruptKEF2 i}): real_secret i =
+  lemma_honest_corrupt i;
+  if model then
+    let t : s:ideal_or_real (mref_secret u i) (real_secret i) {safeKEF2 i <==> Ideal? s} = p in
+    Real?.v t
+  else p
+
+type ext2 (u: usage info) (i:regid) = i':regid{i' == Derive i "" Extract} & salt2 u i'
+
+val coerce_salt2:
+  #u: usage info ->
+  i: regid ->
+  a: info {a == get_info i} ->
+  raw: lbytes (secret_len a) ->
+  ST (ext2 u i)
+  (requires fun h0 -> idealKEF2 ==> corrupt i)
+  (ensures fun h0 p h1 -> (*TBC*) True)
+
+let coerce_salt2 #u i a raw =
+  let i', honest' = register_derive i "" Extract in
+  lemma_corrupt_invariant i "" Extract;
+  (| i', real_salt2 #u #i' raw |)
+
+let ideal_salt2 (#u: usage info) (#i:regid) (t: mref_secret u i{safeKEF2 i}) : salt2 u i =
+  let t : s:ideal_or_real (mref_secret u i) (real_secret i) {safeKEF2 i <==> Ideal? s} = Ideal t in
+  assert(model); t
+
+let salt2_ideal (#u: usage info) (#i:regid) (p:salt2 u i {safeKEF2 i}): mref_secret u i =
+  let t : s:ideal_or_real (mref_secret u i) (real_secret i) {safeKEF2 i <==> Ideal? s} = p in
+  Ideal?.v t
+
+val create_salt2:
+  #u: usage info ->
+  i: regid ->
+  a: info {a == get_info i} ->
+  ST (i':regid{i' == Derive i "" Extract} & salt2 u i')
   (requires fun h0 -> True)
   (ensures fun h0 p h1 -> (*TBC*) True)
-let create_salt2 #u i a = 
-  if honest i then 
-    let t' = secret u (Derive i "" Extract) in 
-    let r: mref_secret u (Derive i "" Extract) = Monotonic.RRef.m_alloc there None in // better style or library call? 
-    let r: salt2 u i = r in
-    r
-  else 
-    coerce_salt2 #u i a (sample (secret_len a)) 
 
-let saltp2 (u:usage info): pkg info (ii get_info) = Pkg 
-  (salt2 u)
+let create_salt2 #u i a =
+  let i', honest' = register_derive i "" Extract in
+  let honest = get_honest i in
+  lemma_corrupt_invariant i "" Extract;
+  if flag_KEF2 && honest' then
+    let t' = secret u i' in
+    let r: mref_secret u i' = MR.m_alloc #(option t') #(ssa #t') there None in
+    (| i', ideal_salt2 #u #i' r |)
+  else
+    (| i', real_salt2 #u #i' (sample (secret_len a)) |)
+
+let saltp2 (u:usage info): pkg info (ii get_info) = Pkg
+  (ext2 u)
   secret_len
-  create_salt2 
+  idealKEF2
+  create_salt2
   coerce_salt2
 
 /// HKDF.Extract(key=s, materials=0) idealized as a single-use PRF.
 /// The salt is used just for extraction, hence [u] here is for the extractee.
 /// Otherwise the code is similar to [derive], with different concrete details
-val extract2: 
+val extract2:
   #u: usage info ->
-  #i: id ->
-  s: salt2 u i -> 
+  #i: regid ->
+  s: ext2 u i ->
   a: info {a == get_info i} ->
-  ST (secret u (Derive i "" Extract))
+  ST (secret u (dfst s))
     (requires fun h0 -> True)
     (ensures fun h0 p h1 -> (*TBC*) True)
 
-let extract2 #u #i s a = 
-  let i' : id = Derive i "" Extract in 
+let extract2 #u #i e2 a =
+  let (| i', s |) = e2 in
+  let honest' = get_honest i' in
+  assert(wellformed_id i');
   assert(a = get_info i');
-  if (* Flags.extract0 && *) honest i 
-  then 
-    let s: mref_secret u i' = s in 
-    match Monotonic.RRef.m_read s with
+  assume(idealKDF ==> idealKEF2); // TODO
+  if flag_KEF2 && honest' then
+    let k: mref_secret u i' = salt2_ideal s in
+    match MR.m_read k with
     | Some extract -> extract
-    | None -> 
-        let extract = create u i' a in 
-        //TODO framing 
-        // Monotonic.RRef.m_write k extract; 
-        extract 
-  else 
-    let raw = HKDF.extract #(a.ha) s (Hashing.zeroHash a.ha) in 
-    assume(honest i' ==> honest i); //17-10-31 TODO with Antoine
+    | None ->
+        let extract = create u i' a in
+        let mrel = ssa #(secret u i') in
+        let () =
+          MR.m_recall k;
+          let h = get() in
+          assume (MR.m_sel h k == None); // TODO framing of call to create
+          assume (mrel None (Some extract)); // TODO Fix the monotonic relation
+          MR.m_write k (Some extract) in
+        extract
+  else
+    let k = salt2_real s in
+    let raw = HKDF.extract #(a.ha) (Hashing.zeroHash a.ha) k in
     coerce u i' a raw
-
-
-
 
 
 /// module KeySchedule
@@ -1083,18 +1402,18 @@ let get_keylen (i:id) = some_keylen
 inline_for_extraction
 let u_default:  usage info = fun lbl -> Use keylen get_keylen (rp (ii get_keylen)) (fun i a ctx -> some_keylen)
 
-// p:pkg ii & (i:id -> ctx:info i -> j:id & p.use j)  = 
+// p:pkg ii & (i:id -> ctx:info i -> j:id & p.use j)  =
 
-assume val get_aeadAlg: i:id -> aeadAlg 
+assume val get_aeadAlg: i:id -> aeadAlg
 let derive_aea (lbl:label) (i:id) (a:info) (ctx:context{wellformed_id (Derive i lbl ctx)}):  a': aeadAlg {a' == get_aeadAlg (Derive i lbl ctx)}
 =
   //fixme! should be extracted from a
   get_aeadAlg (Derive i lbl ctx)
- 
+
 inline_for_extraction
-let u_traffic: usage info = 
-  fun (lbl:label) -> 
-  match lbl with 
+let u_traffic: usage info =
+  fun (lbl:label) ->
+  match lbl with
   | "ClientKey" | "ServerKey" -> Use aeadAlg get_aeadAlg (mp (ii get_aeadAlg)) (derive_aea lbl)
   | _ -> u_default lbl
 
@@ -1102,30 +1421,30 @@ let u_traffic: usage info =
 // #set-options "--print_universes --print_implicits"
 
 let derive_info (lbl:label) (i:id) (a:info) (ctx:context{wellformed_id (Derive i lbl ctx)}): a': info {a' == get_info (Derive i lbl ctx)}
-= 
-  let Info ha o = a in 
+=
+  let Info ha o = a in
   assume false; //17-11-02 lemma needed?
-  match ctx with 
+  match ctx with
   | ExpandLog log hv -> Info ha (Some (Log log hv))
   | _ -> Info ha o
 
 // 17-10-20 this causes a loop, as could be expected.
 inline_for_extraction
-let rec u_master_secret (n:nat ): Tot (usage info) (decreases (%[n; 0])) = 
-  fun lbl -> match lbl with 
+let rec u_master_secret (n:nat ): Tot (usage info) (decreases (%[n; 0])) =
+  fun lbl -> match lbl with
   | "traffic" -> Use info get_info (pp u_traffic) (derive_info lbl)
-  | "resumption" -> 
-    if n > 0 
+  | "resumption" ->
+    if n > 0
     then Use info get_info (pskp (u_early_secret (n-1))) (derive_info lbl)
     else u_default lbl
   | _ -> u_default lbl
-and u_handshake_secret (n:nat): Tot (usage info) (decreases (%[n; 1])) =  
-  fun lbl -> match lbl with 
+and u_handshake_secret (n:nat): Tot (usage info) (decreases (%[n; 1])) =
+  fun lbl -> match lbl with
   | "traffic" -> Use info get_info (pp u_traffic) (derive_info lbl)
   | "salt" -> Use info get_info (saltp2 (u_master_secret n)) (derive_info lbl)
   | _ -> u_default lbl
-and u_early_secret (n:nat): Tot (usage info) (decreases (%[n;2])) = 
-  fun lbl -> match lbl with 
+and u_early_secret (n:nat): Tot (usage info) (decreases (%[n;2])) =
+  fun lbl -> match lbl with
   | "traffic" -> Use info get_info (pp u_traffic) (derive_info lbl)
   | "salt" -> Use info get_info (saltp (u_handshake_secret n)) (derive_info lbl)
   | _ -> u_default lbl
@@ -1134,31 +1453,31 @@ and u_early_secret (n:nat): Tot (usage info) (decreases (%[n;2])) =
 /// One cheap trick is to store a PSK only when it enables resumption.
 
 (* not necessary?
-type shape = | 
-  | Preshared0: nat 
+type shape = |
+  | Preshared0: nat
   | Derive0: shape -> label -> shape
 
-type secret (ui: id -> usage info) (i: id) 
-type secret (u: usage info) (ul: label -> usage info) (i: id) 
+type secret (ui: id -> usage info) (i: id)
+type secret (u: usage info) (ul: label -> usage info) (i: id)
 
-let pp (#s: shape) (u: usage s info): pkg info (ii get_info) = Pkg 
-  (secret s u) 
+let pp (#s: shape) (u: usage s info): pkg info (ii get_info) = Pkg
+  (secret s u)
   secret_len
-  (create s u) 
+  (create s u)
   (coerce s u)
 
-val u_of_i: id -> usage info 
+val u_of_i: id -> usage info
 
 /// We replay the key derivation (in reverse constructor order)
-let rec u_of_i i = match i with 
+let rec u_of_i i = match i with
   | Preshared _ _ -> u_early_secret 1
-  | Derive i lbl _ -> 
-       let u = u_of_i i in 
-       let (| info', get_info', pkg', _ |) = u lbl in 
-*)       
+  | Derive i lbl _ ->
+       let u = u_of_i i in
+       let (| info', get_info', pkg', _ |) = u lbl in
+*)
 
 /// Usability? A mock-up of the TLS 1.3 key schedule.
-/// 
+///
 /// Although the usage computes everything at each derivation, each
 /// still requires 3 type annotations to go through... Can we improve
 /// it?
@@ -1171,60 +1490,57 @@ let rec u_of_i i = match i with
 // the caller context and not necessarily useful for the caller.
 
 // Testing normalization works for a parametric depth
-assume val depth:  n:nat {n > 1} 
-let u: usage info = u_early_secret depth 
+assume val depth:  n:nat {n > 1}
+let u: usage info = u_early_secret depth
 
-val ks: unit -> St unit 
+val ks: unit -> St unit
 let ks() =
   let ipsk: id = Preshared Hashing.Spec.SHA1 0 in
   let a = Info Hashing.Spec.SHA1 None in
   let psk0: psk u ipsk = create_psk ipsk a in
-  
-  let i0: id = Derive ipsk "" Extract in 
-  let early_secret: secret u i0 = extract0 psk0 a in
-  let i_traffic0: id = Derive i0 "traffic" Expand in 
-  let early_traffic: secret u_traffic i_traffic0 = derive a early_secret "traffic" Expand in  
-  let i_0rtt: id = Derive i_traffic0 "ClientKey" Expand in
-  let k0: key #(ii get_aeadAlg) i_0rtt = derive a early_traffic "ClientKey" Expand in 
-  let cipher  = encrypt k0 10 in 
 
-  let i_salt1: id = Derive i0 "salt" Expand in 
+  let i0: id = Derive ipsk "" Extract in
+  let early_secret: secret u i0 = extract0 psk0 a in
+  let (| i_traffic0, early_traffic |) = derive a early_secret "traffic" Expand in
+  assert(i_traffic0 == Derive i0 "traffic" Expand);
+  admit()
+
+
+  let i_0rtt: id = Derive i_traffic0 "ClientKey" Expand in
+  let k0: key #(ii get_aeadAlg) i_0rtt = derive a early_traffic "ClientKey" Expand in
+  let cipher  = encrypt k0 10 in
+
+  let i_salt1: id = Derive i0 "salt" Expand in
   let salt1:  salt (u_handshake_secret depth) i_salt1 = derive a early_secret "salt" Expand in
   let g = CommonDH.default_group in
-  let x = initI g in 
-  let gX = CommonDH.pubshare x in
-  let (| gY, hs_secret |) = extractR salt1 a g gX in 
-  let idh = IDH gX gY in 
-  let i1: id = Derive i_salt1 "" (ExtractDH idh) in 
-  let hs_secret: secret (u_handshake_secret depth) i1= hs_secret in 
+  let x = initI g in
+  let gX = (| g, CommonDH.ipubshare x |) in
+  let (| i_gY, hs_secret |) = extractR salt1 a gX in
+  let (| _, gY |) = i_gY in
+  let idh = IDH gX gY in
+  let i1: id = Derive i_salt1 "" (ExtractDH idh) in
+  let hs_secret: secret (u_handshake_secret depth) i1= hs_secret in
   let i_traffic1: id = Derive i1 "traffic" Expand  in
-  let hs_traffic: secret u_traffic i_traffic1 = derive a hs_secret "traffic" Expand in 
-  let k1: key #(ii get_aeadAlg) (Derive i_traffic1 "ServerKey" Expand) = derive a hs_traffic "ServerKey" Expand in 
-  let cipher  = encrypt k1 11 in 
-  
-  let i_salt2: id = Derive i1 "salt" Expand in 
-  let salt2: salt (u_master_secret depth) i_salt2 = 
-    //Subtyping check failed; expected type 
-    // IK.salt (IK.u_master_secret IK.depth) i_salt2; got type 
-    // IK.derived_key (IK.u_handshake_secret IK.depth) i1 "salt" IK.Expand
-    // derive a hs_secret "salt" Expand in 
-    magic () in //NS: magic is better because it doesn't admit the continuation. CF: Ok; good to know. But the two types above are equal, right? 
-    //admit() in //17-11-02 not sure why this one is now failing 
-  let i2: id = Derive i_salt2 "" Extract in 
-  let master_secret: secret (u_master_secret depth) i2 = extract2 #(u_master_secret depth) #i_salt2 
-    (magic ()) //NS: used to be (* salt2 *)  //expected type IK.salt2 (IK.u_master_secret IK.depth) i_salt2; got type IK.salt (IK.u_master_secret IK.depth) i_salt2
-    a in 
-  let i3: id = Derive i2 "resumption" Expand in 
-  let rsk: psk (u_early_secret (depth - 1)) i3  = derive a master_secret "resumption" Expand in 
+  let hs_traffic: secret u_traffic i_traffic1 = derive a hs_secret "traffic" Expand in
+  let k1: key #(ii get_aeadAlg) (Derive i_traffic1 "ServerKey" Expand) = derive a hs_traffic "ServerKey" Expand in
+  let cipher  = encrypt k1 11 in
+
+  let i_salt2: id = Derive i1 "salt" Expand in
+  let salt2: salt (u_master_secret depth) i_salt2 = admit() in //17-11-02 not sure why this one is now failing // derive a hs_secret "salt" Expand in
+  let i2: id = Derive i_salt2 "" Extract in
+  let master_secret: secret (u_master_secret depth) i2 = extract2 #(u_master_secret depth) #i_salt2 salt2 a in
+  let i3: id = Derive i2 "resumption" Expand in
+  let rsk: psk (u_early_secret (depth - 1)) i3  = derive a master_secret "resumption" Expand in
   let i4: id = Derive i3 "" Extract in
   let next_early_secret: secret (u_early_secret (depth -1)) i4 = extract0 rsk a in
   ()
 
-(* --- 
+
+(* ---
 
 let i3 = Extract0 (Derived i2 "resumption")
-let rsk = derive master_secret "resumption" 
-// #(u_master_secret depth ) #i2 
+let rsk = derive master_secret "resumption"
+// #(u_master_secret depth ) #i2
 val next_early_secret: secret (u_early_secret (depth - 1)) i3 a
 let next_early_secret = extract0 rsk
 
@@ -1237,35 +1553,35 @@ let psk0: psk #u ipsk  a = create_psk ipsk a
 
 let i0 = Derive ipsk "" Extract
 let a0 = Info #i0 Hashing.Spec.SHA1 None
-let early_secret: secret u i0 a0 = extract0 psk0 
+let early_secret: secret u i0 a0 = extract0 psk0
 
-let i_traffic0 = Derive i0 "traffic" Expand 
+let i_traffic0 = Derive i0 "traffic" Expand
 let a_traffic0 = Info #i_traffic0 Hashing.Spec.SHA1 None
 val early_traffic: secret u_traffic i_traffic0 a_traffic0
-let early_traffic = derive early_secret "traffic" Expand 
+let early_traffic = derive early_secret "traffic" Expand
 // not sure where to add the loginfo
 
 let i_0rtt = Derive i_traffic0 "ClientKey" Expand
 val k0: key #ii i_0rtt AES_GCM256
-let k0 = derive early_traffic "ClientKey" Expand 
+let k0 = derive early_traffic "ClientKey" Expand
 let cipher  = encrypt k0 10
 
-let i_salt1 = Derive i0 "salt" Expand 
+let i_salt1 = Derive i0 "salt" Expand
 let a_salt1 = Info #i_salt1 Hashing.Spec.SHA1 None
-val salt1:  salt (u_handshake_secret depth) i_salt1 a_salt1 
+val salt1:  salt (u_handshake_secret depth) i_salt1 a_salt1
 let salt1  = derive early_secret "salt" Expand
 
 
 let g = CommonDH.default_group
-//let x: CommonDH.sh = initI g 
-let x = CommonDH.keygen g 
+//let x: CommonDH.sh = initI g
+let x = CommonDH.keygen g
 let gX = CommonDH.pubshare x
 let gY: CommonDH.share g = admit()
 let dhe_id: id_dhe = Some (| g, gX, gY |)
 
 let i1 = Extract1 (Derived i0 "salt") dhe_id
 
-// we really need [let u_extract1 = u_handshake_secret depth] to go past this point. 
+// we really need [let u_extract1 = u_handshake_secret depth] to go past this point.
 
 val hs_secret : secret (u_handshake_secret depth) i1 a
 let hs_secret = extractI salt1 g x gY
@@ -1274,21 +1590,21 @@ val hs_traffic: secret u_traffic (Derived i1 "traffic") a
 let hs_traffic = derive hs_secret "traffic"
 
 val k1: key #ii (Derived (Derived i1 "traffic") "ServerKey") AES_GCM256
-let k1 = derive hs_traffic "ServerKey" 
+let k1 = derive hs_traffic "ServerKey"
 let cipher' = encrypt k1 11
 
 val salt2:  salt ii (u_master_secret depth) (Derived i1 "salt") a
 let salt2  = derive hs_secret "salt"
 
-let i2 = Extract2 (Derived i1 "salt")  
+let i2 = Extract2 (Derived i1 "salt")
 val master_secret: secret (u_master_secret depth) i2 a
-let master_secret = extract2 salt2 
+let master_secret = extract2 salt2
 
 val rsk: psk #ii #(u_early_secret (depth - 1)) (Derived i2 "resumption") a
 
 let i3 = Extract0 (Derived i2 "resumption")
-let rsk = derive master_secret "resumption" 
-// #(u_master_secret depth ) #i2 
+let rsk = derive master_secret "resumption"
+// #(u_master_secret depth ) #i2
 val next_early_secret: secret (u_early_secret (depth - 1)) i3 a
 let next_early_secret = extract0 rsk
 
@@ -1307,21 +1623,21 @@ let next_early_secret = extract0 rsk
 /// Underlying functionality: create takes explicit random input
 /// idealizes (at most) when its input is freshly sampled.
 ///
-/// real: at creation-time, 
-/// table: label -> 
-/// 
-/// - how to benefit from the create post-condition? explicit? 
-/// 
+/// real: at creation-time,
+/// table: label ->
+///
+/// - how to benefit from the create post-condition? explicit?
+///
 
- 
+
 // let k0 = create_psk 0 //: secret (u depth) ii (Secret 0) = create (u depth) ii (Secret 0)
 // let i1 = Derived (Preshared 0) "secret" (* this seems to help normalization *)
-// let k1: secret (u (depth-1)) ii i1  = derive k0 "secret" 
-// let k2: key #ii (Derived i1 "aead") = derive k1 "aead" 
+// let k1: secret (u (depth-1)) ii i1  = derive k0 "secret"
+// let k2: key #ii (Derived i1 "aead") = derive k1 "aead"
 // let cipher  = encrypt k2 42
 // let k3: list nat  = derive k1 "raw"
 //
-// let k1' = derive k0 "secret" 
+// let k1' = derive k0 "secret"
 // let k2' = derive #(u 22)  k1'  "aead"  // the type is not normalized; the key is not usable.
 
 --- *)
