src/tls/ideal-flags/Flags.fst
@@ -9,13 +9,14 @@ assume val debug_HS : bool
 assume val debug_HSL : bool
 assume val debug_KS : bool
 assume val debug_NGO : bool
-assume val debug_QUIC : bool 
-assume val debug_Record : bool 
+assume val debug_QUIC : bool
+assume val debug_Record : bool
 assume val debug_TLS : bool
 
+assume val model: bool // scaffolding
 assume val ideal_KEF : bool
-assume val ideal_Nonce : bool 
-assume val ideal_Sig : bool 
-assume val ideal_PMS : bool 
-assume val ideal_PRF : bool 
+assume val ideal_Nonce : bool
+assume val ideal_Sig : bool
+assume val ideal_PMS : bool
+assume val ideal_PRF : bool
 assume val ideal_AEAD: bool
